\subsection{The 1-mesa special case}
\label{sec:1-mesa}

The case of the stability of a one mesa solution with Neumann boundary conditions will now by considered. This has to be done separately as the Floquet theory used in the $K-$ mesa case is for $j=1,\cdots,K-1$, and so does not include the case for $K=1$.

The analysis is analogous to what was previously done for $K-$mesas, and we will start at \eqref{eqn:lam}, which we write as
% 
\begin{equation}
% \label{eqn:lam}
	\begin{split}
	\Ep^{-1}\bar{\lA}\kA_0\begin{pmatrix}c_+\\c_-\end{pmatrix}
   &=
	\begin{pmatrix} -\psi(l) \\ \psi(-l) \end{pmatrix}
	 +v_x(l) \begin{pmatrix}c_+\\c_-\end{pmatrix}\\
	\begin{pmatrix}c_+\\c_-\end{pmatrix},
	\end{split}
\end{equation}
% 
with 
% 
\[
  v_x(l) = \left(\frac{\Ep}{\DD}\right)\frac{g_-g_+L}{g_--g_+},
\]
% 
and $\psi(x)$ satisfies
% 
\begin{equation}
\label{eqn:psi2}
\begin{split}
  \psi(x)_{xx}-\sI^2\psi &= \frac{c_+\Ep}{\DD}(g_+-g_-)\dE(x-l) - \frac{c_-\Ep}{\DD}(g_+-g_-)\dE(x+l),\\
  &\psi'(-L) = \psi'(L) = 0.
\end{split}
\end{equation}
% 

Analogous with \eqref{eqn:psi_full}, we obtain that 
% 
\begin{equation*}
% \label{eqn:psi_full}
	\begin{split}
	\psi(x) &= \left\{
	\begin{matrix}
	  \psi(-l)\dfrac{\cosh[\sI_-(x+L)]}{\cosh[\sI_-(L-l)]},&-L<x<-l,\\
	  \psi(-l)\dfrac{\sinh[\sI_+(l-x)]}{\sinh(2\sI_+l)} + \psi(l)\dfrac{\sinh[\sI_+(x+l)]}{\sinh(2\sI_+l)},&-l<x<l,\\
	  \psi(l)\dfrac{\cosh[\sI_-(L-x)]}{\cosh[\sI_-(L-l)]},&l<x<L,\\
	\end{matrix}\right.
	\end{split}
\end{equation*}
% 
with $s = \frac{\Ep}{\DD}(g_+-g_-)$.


The unknowns $\psi(\pm l)$ are to be found by satisfying the jump conditions $\Big.\psi_x\Big|_{-l^-}^{-l^+} = - c_-s$, and $\Big.\psi_x\Big|_{l^-}^{l^+} = c_+s$, hence we get
% 
\begin{equation*}
% \label{eqn:psi_full}
	\begin{split}
	  \psi(l)\big[\sI_-\tanh[\sI_-(L-l)] + \sI_+\coth(2\sI_+l)\big] - \psi(-l)\sI_+\csch(2\sI_+l) &= -c_+s,\\
	  \psi(l)\sI_+\csch(2\sI_+l) - \psi(-l)\big[\sI_+\coth(2\sI_+l)  + \sI_-\tanh[\sI_-(L-l)]\big] &= -c_-s.
	\end{split}
\end{equation*}
% 

We can write this as the linear system
% 
\[
  \begin{pmatrix} d&e\\e&d \end{pmatrix}\begin{pmatrix} \psi(l)\\-\psi(-l) \end{pmatrix} = 
  -s \begin{pmatrix} c_+\\c_- \end{pmatrix},\qquad
  G \equiv \begin{pmatrix} d&e\\e&d \end{pmatrix},
\]
% 
where
% 
\[
  \begin{split}
    d&\equiv \sI_-\tanh[\sI_-(L-l)] + \sI_+\coth(2\sI_+l),\\
	e&\equiv \sI_+\csch(2\sI_+l).
  \end{split}
\]
% 

Inverting $G$ and substituting into \eqref{eqn:psi2}, we get
% 
\begin{equation*}
% \label{eqn:psi_full}
	\begin{split}
	  \frac{\Ep^{-1}\bar{\lA}\kA_0}{s}\begin{pmatrix} c_+\\c_- \end{pmatrix} = \frac{v_x(l)}{s}\begin{pmatrix} c_+\\c_- \end{pmatrix} + G^{-1}\begin{pmatrix} c_+\\c_- \end{pmatrix},
	\end{split}
\end{equation*}
% 
with $v_x(l)/s$ as in \eqref{eqn:vx},
% 
\[
  \frac{v_x(l)}{s} = \frac{\Ep}{\DD}\frac{g_-g_+L}{g_+-g_-}\frac{\DD}{\Ep(g_+-g_-)} = \frac{g_-g_+L}{(g_+-g_-)^2} = \left(1-\frac{L}{l} \right)\frac{l^2}{L^2}L,
\]
% 
and similarly,
% 
\[
  \frac{\Ep^{-1}\bar{\lA}\kA_0}{s} = \frac{\Ep^{-1}\bar{\lA}\kA_0}{(\Ep/\DD)(g_+-g_-)} = - \frac{\DD}{\Ep^2g_-}\bar{\lA}\kA_0\left(\frac{l}{L}\right).
\]
% 

Putting it all together, we conclude that
% 
\begin{equation}
\label{eqn:general_lambda}
  G^{-1}\begin{pmatrix} c_+\\c_- \end{pmatrix} + \left(1-\frac{L}{l} \right)\frac{l^2}{L^2}L\begin{pmatrix} c_+\\c_- \end{pmatrix} = - \frac{\DD}{\Ep^2g_-}\bar{\lA}\kA_0\left(\frac{l}{L}\right)\begin{pmatrix} c_+\\c_- \end{pmatrix},
\end{equation}
% 
with 
% 
\[
  G^{-1} = \frac{1}{d^2-e^2}\begin{pmatrix} d&-e\\-e&d \end{pmatrix}.
\]
%

Thus, the stability of a single mesa is governed by \eqref{eqn:general_lambda}. 

\begin{remark}
As a sanity check, we need to show that \eqref{eqn:general_lambda} evaluated for the GMS system yields an equivalent equation as the matrix problem in equation $(5.15)$ of \cite{kolokolnikov_stability_2005}. 

Similarly, we also need to show that the general $K-$mesa matrix problem given in \eqref{eqn:ceqn1} is also equivalent in the GMS case to the previously computed system in \eqref{eqn:Kmesa_gms}.
\end{remark}

We have from $(5.15)$ of \cite{kolokolnikov_stability_2005} that
% 
\begin{equation}
\label{eqn:lam_old}
  \left[\frac{L}{2}(1-L)I-\hat{G}^{-1} \right]\hat{c}=\frac{\aL}{\Ep^2}\bar{\lA}\hat{c},\qquad\text{with }\hat{c} = \begin{pmatrix} c_l\\c_r \end{pmatrix},
\end{equation}
% 
where $L$ is the width of the mesa, and the domain has constant length 1; and
% 
\[
  \hat{G}^{-1} = \frac{1}{d^2-e^2}\begin{pmatrix} d&e\\e&d \end{pmatrix},\qquad \aL\equiv\frac{2\bE L\DD}{w_+^2},\qquad \beta = \int_{-\infty}^{\infty}w'^2dy.
\]
%

\begin{remark}
Notice that in the formulation for $\vec{c}$ in \eqref{eqn:phi_aprox1} and \eqref{eqn:phi_aprox2}, when compared to $\hat{c}$, we have that $c_l=c_-$, but $c_r=-c_+$.

Rewriting \eqref{eqn:lam_old} in the notation we have been using, we have that $L=2l$ is the width of the mesa, and we have
\end{remark}
 % 
\begin{equation}
\label{eqn:lam_old2}
  \left[\hat{G}^{-1}-l(1-2l)I \right]\hat{c}=-\frac{\aL}{\Ep^2}\bar{\lA}\hat{c},
\end{equation}
% 
with $\aL =\frac{2\bE(2l)\DD}{w_+^2}$.

Now, in our formulation, if we restrict it to the case $L=1/2$ (domain length 1), we obtain
 % 
\begin{equation}
\label{eqn:lam_new1}
  \left[{G}^{-1}-l(1-2l)I \right]\vec{c}=-\frac{\DD\kA_0(2l)}{\Ep^2g_-}\bar{\lA}\vec{c}.
\end{equation}
% 

For the left hand side, we expand \eqref{eqn:lam_old2} as
 % 
\begin{equation*}
\begin{split}
% \label{eqn:lam_old2}
  -\frac{1}{d^2-e^2}\left[dc_l+ec_r \right]+l(1-2l)c_l &= \frac{\aL}{\Ep^2}\bar{\lA}c_l,\\
  \frac{1}{d^2-e^2}\left[dc_r+ec_l \right]-l(1-2l)c_r &= -\frac{\aL}{\Ep^2}\bar{\lA}c_r.
\end{split}
\end{equation*}
% 

Interchanging the rows, we can write this as
% 
\[
  \frac{1}{d^2-e^2}\begin{pmatrix} d&-e\\-e&d \end{pmatrix}\begin{pmatrix} c_r\\-c_l \end{pmatrix} -l(1-2l)\begin{pmatrix} c_r\\-c_l \end{pmatrix} = -\frac{\aL}{\Ep^2}\bar{\lA}\begin{pmatrix} c_r\\-c_l \end{pmatrix},
\]
% 
and since $c_r = -c_+$, and $c_l = c_-$, this system is equivalent to \eqref{eqn:lam_new1}, provided that the right hand sides match, and that the $d$ and $e$ values are consistent.

Thus, we only need to show that 
% 
\[
  \aL = \frac{4\bE l\DD}{w_+^2}= \frac{2l\kA_0\DD}{g_-},
\]
% 
or, more succinctly, that
% 
\[
  \frac{2\bE}{w_+^2}=\frac{\kA_0}{g_-}, 
\]
% 
where
% 
\[
  \bE = \int_{-\infty}^{\infty}w'^2dy,\quad U_0=\VV w(y),\quad \kA_0 = \frac{\int_{-\infty}^{\infty}(U_0')^2dy}{\int_{u_-}^{u_+}f_vdu},\quad g_- = g(u_-,\VV).
\]

For the GMS model we have that 
% 
\[
  \begin{split}
    g(u,v) &= -v+u^2,\\
	f(u,v) &= -u + \frac{u^2}{v(1+\kA u^2)},\qquad\text{and }u_-=0.
  \end{split}
\]
% 

When $v=\VV$, we integrate
% 
\[
  \int_{u_-}^{u_+}f_vdu = -\int_0^{u_+} \frac{u^2}{\VV^2(1+\kA u^2)}du 
\]
% 

Now, we substitute $u=\VV w$, $u_+ = \VV w_+$, and get
% 
\[
  \int_{u_-}^{u_+}f_vdu = -\VV\int_0^{w_+} \frac{w^2}{1+b_0 w^2}dw,\qquad \text{with }b_0=\kA\VV^2 
\]
% 

From the definition of the system in \eqref{eqn:o-w_eqn}, we have that
% 
\[
  w'' - w + \frac{w^2}{1+b_0w^2}=0.
\]
% 

Multiplying by $w'$ and integrating from $y=-\infty$ to $y=\infty$, we get
% 
\[
\begin{split}
  \Big.\frac{w'^2}{2}\Big|_{-\infty}^{\infty} &- \Big.\frac{w^2}{2}\Big|_{-\infty}^{\infty} + \int_{-\infty}^{\infty} \frac{w^2}{1+b_0 w^2}\frac{dw}{dy}dy=0,\\
  &-\frac{w_+^2}{2} + \int_0^{w_+} \frac{w^2}{1+b_0 w^2}dw = 0.
\end{split}
\]
% 

Hence
% 
\[
  \int_0^{w_+} \frac{w^2}{1+b_0 w^2}dw = \frac{w_+^2}{2},
\]
% 
and we can conclude that
% 
\[
  \int_{u_-}^{u_+}f_vdu = -\VV\frac{w_+^2}{2}.
\]
% 

We also calculate that
% 
\[
  \int_{-\infty}^{\infty}(U_0')^2dy = \VV^2\int_{-\infty}^{\infty}(w')^2dy,\qquad g_- = g(u_-,\VV)=-\VV.
\]
% 

We conclude that
% 
\[
  \frac{\kA_0}{g_-} = \frac{\VV^2\int_{-\infty}^{\infty}(w')^2dy}{-\VV(-\VV w_+^2/2)} = \frac{2}{w_+^2}\int_{-\infty}^{\infty}(w')^2dy.
\]

Now, the only thing remaining to ensure compatibility between our result and $(5.15)$ of \cite{kolokolnikov_stability_2005}(??? Their formula for $\tH$ doesn't include the $\lA$ terms???) is to show that the decay rates $\sI_{\pm}$ and $\tH_{\pm}$ are the same.

We have from \eqref{eqn:sigma} that
% 
\begin{equation*}
\begin{split}
	&\quad\sI_{\pm}^2 = m^2  + \frac{\Ep}{\DD}(\kA_{\pm} + \tau\lA), \text{ with}\\
	\kA_+ &\equiv - \left(g_v^+ - \frac{f_v^+}{f_u^+}g_u^+ \right)>0,\\
	\kA_- &\equiv - \left(g_v^- - \frac{f_v^-}{f_u^-}g_u^- \right)>0,
\end{split}
\end{equation*}
% 
and from \eqref{eqn:phi_asym} that $\tH_{\pm}$ is
% 
\begin{equation*}
	\begin{split}
	\tH
   = \left\{
	\begin{matrix}
		\tH_-\equiv\left(m^2+\frac{\Ep(1+\tau\lA)}{\DD}\right)^{1/2},\hspace{0.85in}\\
		\tH_+\equiv\left(m^2+\frac{\Ep(1+\tau\lA)}{\DD}\left(1+\frac{2w_+}{l(w_+-2)} \right)\right)^{1/2}
	\end{matrix}\right.
	\end{split}
\end{equation*}
% 

We have that, for the GMS system,
% 
\[
  u_-=0\quad u_+ = \VV w_+,\quad v=\VV,\quad\text{where }\VV = \frac{1}{w_+^22l}.
\]
% 

Now, we have that $g_u^- = 0$, and $g_v^- = -1$, hence $\kA_- = 1$, and thus $\tH_- = \sI_-$.

Similarly, (??? I've kept the original notation with $\kA$ instead of $\mu$, but at one point I guess I'll have to change it???) since $u_+$ satisfies $f(u_+,\VV)=0$, and thus
% 
\[
  u_+ = \VV(1+\kA u_+^2),
\]
% 
we have,
% 
\[
\begin{split}
\begin{aligned}
  g_u^+ &= 2u_+, && f_u^+ = -1+\frac{2u_+}{\VV(1+\kA u_+^2)^2} = -1 + \frac{2}{1+\kA u_+^2} = -1+\frac{2\VV}{u_+},\\
  g_v^+ &= -1,&& f_v^+ = -\frac{u_+^2}{\VV^2(1+\kA u_+^2)} = -\frac{u_+}{\VV}.
\end{aligned}
\end{split}
\]
% 

We have then
% 
\[
\begin{split}
  \kA_+ &= -\left(g_v^+ - \frac{f_v^+}{f_u^+}g_u^+ \right) = -\left(-1 +  \frac{u_+/\VV}{\frac{2\VV-u_+}{u_+}}2u^+ \right) = 1+\frac{2u_+^3}{\VV u_+-2\VV^2}\\
  & = 1+\frac{2\VV w_+^3}{w_+-2} = 1+\frac{ w_+}{l(w_+-2)}.
\end{split}
\]
 
This shows that $\sI_{\pm} = \tH_{\pm}$, hence the GMS results in $(5.15)$ of \cite{kolokolnikov_stability_2005} are consistent with ours, and thus constitute a particular case of our results.

Our final result is that on a domain $[-L,L]$, with mesa width $2l$, we have
% 
\begin{equation}
\label{eqn:general_lambda2}
  G^{-1}\begin{pmatrix} c_+\\c_- \end{pmatrix} + \left(1-\frac{L}{l} \right)\frac{l^2}{L^2}L\begin{pmatrix} c_+\\c_- \end{pmatrix} = - \frac{\DD}{\Ep^2g_-}\bar{\lA}\kA_0\left(\frac{l}{L}\right)\begin{pmatrix} c_+\\c_- \end{pmatrix},
\end{equation}
% 
where
% 
\[
\begin{split}
\begin{aligned}
  G^{-1} &= \frac{1}{d^2-e^2}\begin{pmatrix} d&-e\\-e&d \end{pmatrix},\\
  d&= \sI_-\tanh[\sI_-(L-l)] + \sI_+\coth(2\sI_+l),\\
  e&= \sI_+\csch(2\sI_+l),\\
  \quad\sI_{\pm}^2 &= m^2  + \frac{\Ep}{\DD}(\kA_{\pm} + \tau\lA),\\
  \kA_+ &= - \left(g_v^+ - \frac{f_v^+}{f_u^+}g_u^+ \right)>0,\\
  \kA_- &= - \left(g_v^- - \frac{f_v^-}{f_u^-}g_u^- \right)>0,\\
  \bar{\lA} &= \lA + \Ep^2m^2,\\
  g_- &= g(u_-,\VV),\\
  \kA_0&=\dfrac{\int_{-\infty}^{\infty}(U_0')^2 dy}{\int_{u_-}^{u_+}f_vdu}.
\end{aligned}
\end{split}
\]
%

It is now convenient to define
% 
\[
  \vA = -\frac{\DD}{g_-}\kA_0\left(\frac{l}{L} \right).
\]
% 
Then, with $I$ the identity matrix, we can rewrite \eqref{eqn:general_lambda2} as
% 
\[
  \left(G^{-1} + \left(1-\frac{L}{l} \right)\frac{l^2}{L^2}LI - m^2\vA I\right)\vec{c} = \frac{\vA}{\Ep^2}\lA\vec{c}
\]
% 

The eigenpairs of the system are then
% 
\begin{equation}
\begin{split}
\label{eqn:lam_pm}
  \lA_{\pm} &= \frac{\Ep^2}{\vA}\left[\oM_{\pm} + \left(1-\frac{L}{l} \right)\frac{l^2}{L^2}L - m^2\vA \right],\\
  \vec{c}_{\pm} &= \begin{pmatrix} 1\\ \mp1 \end{pmatrix},
\end{split}
\end{equation}
% 
with $\oM_{\pm}$ the eigenvalues of $G^{-1}$, given by
% {
\[
  \begin{split}
    \oM_+ &= \frac{1}{d-e} = [\sI_-\tanh[\sI_-(L-l)]+\sI_+\tanh(l\sI_+)]^{-1},\\
	\oM_- &= \frac{1}{d+e} = [\sI_-\tanh[\sI_-(L-l)]+\sI_+\coth(l\sI_+)]^{-1},\\
  \end{split}
\]

The $(\lA_+,\vec{c}_+)$ eigenpair corresponds then to the breather mode, and the $(\lA_-,\vec{c}_-)$ is the zigzag mode.

\begin{itemize}
  \item{ The case $m\neq0$, $\tau=O(1)$:

	We have that irrespective of the sign of $\vA$, for $m$ sufficiently large both, we will have that $\lA_{\pm}<0$, i.e., the stripe is stable to short wavelength perturbations in the y-direction.

	We have that $\oM_{\pm}>0$, and in fact as $L\rightarrow\infty$ we have $\oM_{\pm}\sim\frac{1}{2m}$. Given that $1-L/l<0$, with the ratio $L/l$ remains constant when only the domain length $L$ is increased, we have that on a small enough domain the stripe will always be stable, and that there will be a critical length $L$ beyond which the stripe will become unstable.
}

  \item{ The case $m=0$, $\tau=O(1)$:

	When $\Ep\rightarrow0$ we have that $\sI_{\pm}\rightarrow0$. For the zigzag mode ($\lA_-$), we have that
	\[
	  \sI_+\coth(\sI_+l)=\frac{\sI_+}{\tanh(\sI_+l)}\sim\frac{1}{l(1-\frac{\sI^2l^2}{3})}\sim\frac{1}{l}+O(\sI_+^2),
	\]
	and since $\sI_-\tanh[\sI_-(L-l)]\sim\sI_-^2(L-l)$, we have
	\[
	  \oM_-\sim \left[\sI_-^2(L-l) + \frac{1}{l} + O(\sI_+^2) \right]^{-1} = l + O(\sI_+^2,\sI_-^2).
	\]

	We conclude that for $m=0$ we have
	\begin{equation*}
	  \lA_-\simeq \frac{\Ep^2}{\vA}\left[\left(1 - \frac{L}{l} \right)\frac{l^2}{L^2}L + l + O(\sI_+^2,\sI_-^2)\right] \sim \frac{\Ep^2}{\vA}\left[\left(\frac{l^2}{L^2}\right)L + O(\sI_+^2,\sI_-^2)\right],
	\end{equation*}
	and stability is guaranteed for this mode when $\vA<0$

\begin{remark}
  When $\tau\ll1$ this analysis is consistent provided that the term in $\oM_{\pm}$ $\Ep\tau\lA\ll1$. Since this shows that $\lA=O(\Ep^2)$, the condition for self-consistency is that $\tau\ll O(\Ep^3)$.
\end{remark}

	Now, for the breather mode $\lA_+$, we have that
	\[
	  \oM_+\sim \frac{1}{\sI_-^2(L-l) + \sI_+^2l} = \frac{1}{\sI_-^2L + l(\sI_+^2-\sI_-^2)}.
	\]

	Since $\sI_-^2 = \frac{\Ep}{\DD}(\kA_-+\tau\lA)$, and $\sI_+^2-\sI_-^2 = \frac{\Ep}{\DD}(\kA_+-\kA_-)$, we have that
	\[
	  \oM_+^2\sim\frac{\DD}{\Ep L\left[(\kA_-+\tau\lA) + \frac{l}{L}(\kA_+-\kA_-) \right]}.
	\]
	
	In terms of the breather eigenvalue, this yields that
	\begin{equation*}
	  \lA_+ = \frac{\Ep^2}{\vA}\left[\oM_+ + \left(1-\frac{L}{l} \right)\frac{l^2}{L^2}L \right] \sim \frac{\Ep\DD}{L\vA}\frac{1}{(\kA_-+\tau\lA) + \frac{l}{L}(\kA_+-\kA_-)}.
	\end{equation*}

	Notice again that since $l/L<1$ we have stability of this mode provided that $\vA<0$.

\begin{remark}
  Notice that the breather eigenvalue $\lA_+ = O(\Ep)$, while the zigzag eigenvalue $\lA_-=O(\Ep^2)$.

  The consistency condition for the breather case is that $0<\tau<O(\Ep^{-1})$, since $\lA_+=O(\Ep,\tau\lA)$.
\end{remark}

}
\end{itemize}



